progs/fupd.v
@@ -1,0 +1,255 @@
+Require Import VST.msl.ghost.
+Require Import VST.msl.ghost_seplog.
+Require Import VST.msl.sepalg_generators.
+Require Import VST.veric.compcert_rmaps.
+Require Import VST.progs.ghosts.
+Require Import VST.progs.conclib.
+Require Import VST.progs.invariants.
+Import Ensembles.
+
+(* Where should this sit? *)
+
+Definition except0 P := P || |>FF.
+
+Definition timeless P := |>P |-- except0 P.
+
+Definition timeless' (P : mpred) := forall (a a' : rmap),
+  predicates_hered.app_pred P a' -> age a a' ->
+  predicates_hered.app_pred P a.
+
+Lemma timeless'_timeless : forall P, timeless' P -> timeless P.
+Proof.
+  unfold timeless; intros.
+  change (_ |-- _) with (predicates_hered.derives (|>P) (P || |>FF)); intros ? HP.
+  destruct (level a) eqn: Ha.
+  - right; intros ? ?%laterR_level; omega.
+  - left.
+    destruct (levelS_age a n) as [b [Hb]]; auto.
+    specialize (HP _ (semax_lemmas.age_laterR Hb)).
+    eapply H; eauto.
+Qed.
+
+Lemma address_mapsto_timeless : forall m v sh p, timeless (res_predicates.address_mapsto m v sh p).
+Proof.
+  intros; apply timeless'_timeless.
+  repeat intro.
+  simpl in *.
+  destruct H as (b & [? HYES] & ?); exists b; split; [split|]; auto.
+  intro b'; specialize (HYES b').
+  if_tac.
+  - destruct HYES as (rsh & Ha'); exists rsh.
+    erewrite age_to_resource_at.age_resource_at in Ha' by eauto.
+    destruct (a @ b'); try discriminate; inv Ha'.
+    destruct p0; inv H6; simpl.
+    f_equal.
+    apply proof_irr.
+  - rewrite age1_resource_at_identity; eauto.
+  - rewrite age1_ghost_of_identity; eauto.
+Qed.
+
+Lemma except0_mono : forall P Q, P |-- Q -> except0 P |-- except0 Q.
+Proof.
+  intros; unfold except0.
+  apply orp_left; [apply orp_right1 | apply orp_right2]; auto.
+Qed.
+
+Lemma except0_intro : forall P, P |-- except0 P.
+Proof.
+  intros; unfold except0.
+  apply orp_right1; auto.
+Qed.
+
+Lemma except0_trans : forall P, except0 (except0 P) |-- except0 P.
+Proof.
+  intros; unfold except0.
+  apply orp_left; [|apply orp_right2]; auto.
+Qed.
+
+Lemma except0_timeless : forall P Q, P |-- except0 Q -> timeless P -> |> P |-- except0 Q.
+Proof.
+  intros.
+  eapply derives_trans; eauto.
+  eapply derives_trans, except0_trans.
+  apply except0_mono; auto.
+Qed.
+
+Lemma except0_frame_r : forall P Q, except0 P * Q |-- except0 (P * Q).
+Proof.
+  intros; unfold except0.
+  rewrite distrib_orp_sepcon.
+  apply orp_left; [apply orp_right1 | apply orp_right2]; auto.
+  eapply derives_trans; [apply sepcon_derives, now_later; apply derives_refl|].
+  rewrite <- later_sepcon; apply later_derives.
+  rewrite FF_sepcon; auto.
+Qed.
+
+Lemma except0_bupd_elim : forall P, except0 (|==> except0 P) |-- |==> except0 P.
+Proof.
+  intros; unfold except0.
+  apply orp_left; auto.
+  eapply derives_trans, bupd_intro.
+  apply orp_right2; auto.
+Qed.
+
+Section FancyUpdates.
+
+Context {inv_names : invG}.
+
+Definition fupd (E1 E2 : Ensemble iname) P :=
+  (wsat * ghost_set g_en E1) -* |==> except0 (wsat * ghost_set g_en E2 * P).
+
+Notation "|={ E1 , E2 }=> P" := (fupd E1 E2 P) (at level 62): logic.
+Notation "|={ E }=> P" := (fupd E E P) (at level 62): logic.
+
+Lemma fupd_mono : forall E1 E2 P Q, P |-- Q -> |={E1, E2}=> P |-- |={E1, E2}=> Q.
+Proof.
+  intros; unfold fupd.
+  rewrite <- wand_sepcon_adjoint.
+  rewrite sepcon_comm; eapply derives_trans; [apply modus_ponens_wand|].
+  apply bupd_mono, except0_mono; cancel.
+Qed.
+
+Lemma bupd_fupd : forall E P, |==> P |-- |={E}=> P.
+Proof.
+  intros; unfold fupd.
+  rewrite <- wand_sepcon_adjoint.
+  eapply derives_trans; [apply bupd_frame_r|].
+  rewrite sepcon_comm; apply bupd_mono, except0_intro.
+Qed.
+
+Lemma fupd_frame_r : forall E1 E2 P Q, fupd E1 E2 P * Q |-- fupd E1 E2 (P * Q).
+Proof.
+  intros; unfold fupd.
+  rewrite <- wand_sepcon_adjoint.
+  rewrite sepcon_comm, <- sepcon_assoc.
+  eapply derives_trans; [apply sepcon_derives, derives_refl; apply modus_ponens_wand|].
+  eapply derives_trans; [apply bupd_frame_r|].
+  apply bupd_mono.
+  rewrite <- sepcon_assoc.
+  apply except0_frame_r.
+Qed.
+
+Lemma fupd_intro_mask : forall E1 E2 P (Hdec : forall a, In E2 a \/ ~In E2 a),
+  Included E2 E1 -> P |-- |={E1,E2}=> |={E2,E1}=> P.
+Proof.
+  intros; unfold fupd.
+  rewrite <- wand_sepcon_adjoint.
+  eapply derives_trans, bupd_intro.
+  eapply derives_trans, except0_intro.
+  rewrite ghost_set_subset with (s' := E2) by auto.
+  cancel.
+  rewrite <- wand_sepcon_adjoint.
+  eapply derives_trans, bupd_intro.
+  eapply derives_trans, except0_intro; cancel.
+Qed.
+
+Lemma fupd_trans : forall E1 E2 E3 P, (|={E1,E2}=> |={E2,E3}=> P) |-- |={E1,E3}=> P.
+Proof.
+  intros; unfold fupd.
+  rewrite <- wand_sepcon_adjoint.
+  rewrite sepcon_comm.
+  eapply derives_trans; [apply modus_ponens_wand|].
+  eapply derives_trans; [apply bupd_mono, except0_mono, modus_ponens_wand|].
+  eapply derives_trans, bupd_trans; apply bupd_mono.
+  apply except0_bupd_elim.
+Qed.
+
+Lemma fupd_timeless : forall E P, timeless P -> |> P |-- |={E}=> P.
+Proof.
+  intros; unfold fupd.
+  eapply derives_trans; [apply except0_timeless; auto; apply except0_intro|].
+  rewrite <- wand_sepcon_adjoint.
+  eapply derives_trans; [apply except0_frame_r|].
+  rewrite sepcon_comm.
+  apply bupd_intro.
+Qed.
+
+Lemma fupd_frame_l : forall E1 E2 P Q, P * fupd E1 E2 Q |-- fupd E1 E2 (P * Q).
+Proof.
+  intros; rewrite sepcon_comm, (sepcon_comm P Q); apply fupd_frame_r.
+Qed.
+
+Lemma fupd_bupd : forall E1 E2 P Q, P |-- |==> (|={E1,E2}=> Q) -> P |-- |={E1,E2}=> Q.
+Proof.
+  intros; eapply derives_trans, fupd_trans; eapply derives_trans, bupd_fupd; auto.
+Qed.
+
+Lemma fupd_intro : forall E P, P |-- |={E}=> P.
+Proof.
+  intros; eapply derives_trans, bupd_fupd; apply bupd_intro.
+Qed.
+
+Lemma inv_alloc : forall E P, |> P |-- |={E}=> EX i : _, invariant i P.
+Proof.
+  intros; unfold fupd.
+  rewrite <- wand_sepcon_adjoint.
+  rewrite <- sepcon_assoc, (sepcon_comm _ wsat).
+  eapply derives_trans; [apply sepcon_derives, derives_refl; apply wsat_alloc|].
+  eapply derives_trans; [apply bupd_frame_r|].
+  apply bupd_mono.
+  rewrite sepcon_assoc, (sepcon_comm _ (ghost_set _ _)), <- sepcon_assoc.
+  apply except0_intro.
+Qed.
+
+Corollary make_inv : forall E P Q, P |-- Q -> P |-- |={E}=> EX i : _, invariant i Q.
+Proof.
+  intros.
+  eapply derives_trans, inv_alloc; auto.
+  eapply derives_trans, now_later; auto.
+Qed.
+
+Lemma inv_close_aux : forall E (i : iname) P,
+  ghost_list(P := token_PCM) g_dis (list_singleton i (Some tt)) * invariant i P * |> P *
+  (wsat * ghost_set g_en (Subtract E i))
+  |-- |==> except0 (wsat * (ghost_set g_en (Singleton i) * ghost_set g_en (Subtract E i))).
+Proof.
+  intros.
+  sep_apply (wsat_close i P).
+  eapply derives_trans; [apply bupd_frame_r | apply bupd_mono].
+  rewrite <- sepcon_assoc; apply except0_intro.
+Qed.
+
+Lemma inv_open : forall E i P, In E i ->
+  invariant i P |-- |={E, Subtract E i}=> (|> P) * (|>P -* |={Subtract E i, E}=> emp).
+Proof.
+  intros; unfold fupd.
+  rewrite <- wand_sepcon_adjoint.
+  erewrite ghost_set_remove; eauto.
+  rewrite invariant_dup.
+  sep_apply (wsat_open i P).
+  eapply derives_trans; [apply bupd_frame_r | apply bupd_mono].
+  eapply derives_trans, except0_intro.
+  cancel.
+  rewrite <- !wand_sepcon_adjoint.
+  apply inv_close_aux.
+  { intro; omega. }
+Qed.
+
+(* these last two are probably redundant *)
+Lemma inv_close : forall E i P, In E i ->
+  invariant i P * |> P * ghost_list(P := exclusive_PCM _) g_dis (list_singleton i (Some tt)) |--
+  |={Subtract E i, E}=> TT.
+Proof.
+  intros; unfold fupd.
+  rewrite <- !wand_sepcon_adjoint.
+  rewrite (sepcon_comm _ (ghost_list _ _)), <- 2sepcon_assoc, sepcon_assoc.
+  eapply derives_trans; [apply inv_close_aux|].
+  erewrite (ghost_set_remove _ _ E); eauto.
+  apply bupd_mono, except0_mono; cancel.
+  { intro; omega. }
+Qed.
+
+Lemma inv_access : forall E i P, In E i ->
+  invariant i P |-- |={E, Subtract E i}=> |> P * (|> P -* |={Subtract E i, E}=> TT).
+Proof.
+  intros.
+  eapply derives_trans; [apply inv_open; eauto|].
+  apply fupd_mono; cancel.
+  apply wand_derives; auto.
+  apply fupd_mono; auto.
+Qed.
+
+(* Consider putting rules for invariants and fancy updates in msl (a la ghost_seplog), and proofs
+   in veric (a la own). *)
+
+End FancyUpdates.
